Conversion of AllocBase to new-style

src/ZF/UNITY/AllocBase.thy
@@ -3,70 +3,409 @@
     Author:     Sidi O Ehmety, Cambridge University Computer Laboratory
     Copyright   2001  University of Cambridge
 
-Common declarations for Chandy and Charpentier's Allocator
 *)
 
-AllocBase = Follows + MultisetSum + Guar +
+header{*Common declarations for Chandy and Charpentier's Allocator*}
+
+theory AllocBase = Follows + MultisetSum + Guar:
 
 consts
   tokbag   :: i  (* tokbags could be multisets...or any ordered type?*)
   NbT      :: i  (* Number of tokens in system *)
   Nclients :: i  (* Number of clients *)
-translations
-"tokbag" => "nat" 
-rules
-  NbT_pos  "NbT:nat-{0}"
-  Nclients_pos "Nclients:nat-{0}"
+
+translations "tokbag" => "nat" 
+
+axioms
+  NbT_pos:      "NbT \<in> nat-{0}"
+  Nclients_pos: "Nclients \<in> nat-{0}"
   
-(*This function merely sums the elements of a list*)
-consts tokens     :: i =>i
+text{*This function merely sums the elements of a list*}
+consts tokens :: "i =>i"
        item :: i (* Items to be merged/distributed *)
 primrec 
   "tokens(Nil) = 0"
   "tokens (Cons(x,xs)) = x #+ tokens(xs)"
 
 consts
-  bag_of :: i => i
+  bag_of :: "i => i"
 
 primrec
   "bag_of(Nil)    = 0"
   "bag_of(Cons(x,xs)) = {#x#} +# bag_of(xs)"
 
-(* definitions needed in Client.thy *)
-consts
-  all_distinct0:: i=>i
-  all_distinct:: i=>o
-  
-primrec
+
+text{*Definitions needed in Client.thy.  We define a recursive predicate
+using 0 and 1 to code the truth values.*}
+consts all_distinct0 :: "i=>i"
+ primrec
   "all_distinct0(Nil) = 1"
   "all_distinct0(Cons(a, l)) =
-     (if a:set_of_list(l) then 0 else all_distinct0(l))"
+     (if a \<in> set_of_list(l) then 0 else all_distinct0(l))"
 
-defs
-all_distinct_def
-  "all_distinct(l) == all_distinct0(l)=1"
+constdefs
+  all_distinct  :: "i=>o"
+   "all_distinct(l) == all_distinct0(l)=1"
   
 constdefs  
-  (* coersion from anyting to state *)
-  state_of :: i =>i
-  "state_of(s) == if s:state then s else st0"
+  state_of :: "i =>i" --{* coersion from anyting to state *}
+   "state_of(s) == if s \<in> state then s else st0"
 
-  (* simplifies the expression of programs  *)
+  lift :: "i =>(i=>i)" --{* simplifies the expression of programs*}
+   "lift(x) == %s. s`x"
 
-  lift :: "i =>(i=>i)"
-  "lift(x) == %s. s`x"
+text{* function to show that the set of variables is infinite *}
+consts
+  nat_list_inj :: "i=>i"
+  nat_var_inj  :: "i=>i"
+  var_inj      :: "i=>i"
 
-consts (* to show that the set of variables is infinite *)
-  nat_list_inj :: i=>i
-  nat_var_inj  :: i=>i
-  var_inj :: i=>i
 defs
-  nat_var_inj_def "nat_var_inj(n) == Var(nat_list_inj(n))"
+  nat_var_inj_def: "nat_var_inj(n) == Var(nat_list_inj(n))"
 primrec
   "nat_list_inj(0) = Nil"
   "nat_list_inj(succ(n)) = Cons(n, nat_list_inj(n))"
 
 primrec
   "var_inj(Var(l)) = length(l)"
+
+
+subsection{*Various simple lemmas*}
+
+lemma Nclients_NbT_gt_0 [simp]: "0 < Nclients & 0 < NbT"
+apply (cut_tac Nclients_pos NbT_pos)
+apply (auto intro: Ord_0_lt)
+done
+
+lemma Nclients_NbT_not_0 [simp]: "Nclients \<noteq> 0 & NbT \<noteq> 0"
+by (cut_tac Nclients_pos NbT_pos, auto)
+
+lemma Nclients_type [simp,TC]: "Nclients\<in>nat"
+by (cut_tac Nclients_pos NbT_pos, auto)
+
+lemma NbT_type [simp,TC]: "NbT\<in>nat"
+by (cut_tac Nclients_pos NbT_pos, auto)
+
+lemma INT_Nclient_iff [iff]:
+     "b\<in>Inter(RepFun(Nclients, B)) <-> (\<forall>x\<in>Nclients. b\<in>B(x))"
+apply (auto simp add: INT_iff)
+apply (rule_tac x = 0 in exI)
+apply (rule ltD, auto)
+done
+
+lemma setsum_fun_mono [rule_format]:
+     "n\<in>nat ==>  
+      (\<forall>i\<in>nat. i<n --> f(i) $<= g(i)) -->  
+      setsum(f, n) $<= setsum(g,n)"
+apply (induct_tac "n", simp_all)
+apply (subgoal_tac "Finite(x) & x\<notin>x")
+ prefer 2 apply (simp add: nat_into_Finite mem_not_refl, clarify)
+apply (simp (no_asm_simp) add: succ_def)
+apply (subgoal_tac "\<forall>i\<in>nat. i<x--> f(i) $<= g(i) ")
+ prefer 2 apply (force dest: leI) 
+apply (rule zadd_zle_mono, simp_all)
+done
+
+lemma tokens_type [simp,TC]: "l\<in>list(A) ==> tokens(l)\<in>nat"
+by (erule list.induct, auto)
+
+lemma tokens_mono_aux [rule_format]:
+     "xs\<in>list(A) ==> \<forall>ys\<in>list(A). <xs, ys>\<in>prefix(A)  
+   --> tokens(xs) \<le> tokens(ys)"
+apply (induct_tac "xs")
+apply (auto dest: gen_prefix.dom_subset [THEN subsetD] simp add: prefix_def)
+done
+
+lemma tokens_mono: "<xs, ys>\<in>prefix(A) ==> tokens(xs) \<le> tokens(ys)"
+apply (cut_tac prefix_type)
+apply (blast intro: tokens_mono_aux)
+done
+
+lemma mono_tokens [iff]: "mono1(list(A), prefix(A), nat, Le,tokens)"
+apply (unfold mono1_def)
+apply (auto intro: tokens_mono simp add: Le_def)
+done
+
+lemma tokens_append [simp]: 
+"[| xs\<in>list(A); ys\<in>list(A) |] ==> tokens(xs@ys) = tokens(xs) #+ tokens(ys)"
+apply (induct_tac "xs", auto)
+done
+
+subsection{*The function @{term bag_of}*}
+
+lemma bag_of_type [simp,TC]: "l\<in>list(A) ==>bag_of(l)\<in>Mult(A)"
+apply (induct_tac "l")
+apply (auto simp add: Mult_iff_multiset)
+done
+
+lemma bag_of_multiset:
+     "l\<in>list(A) ==> multiset(bag_of(l)) & mset_of(bag_of(l))<=A"
+apply (drule bag_of_type)
+apply (auto simp add: Mult_iff_multiset)
+done
+
+lemma bag_of_append [simp]:
+    "[| xs\<in>list(A); ys\<in>list(A)|] ==> bag_of(xs@ys) = bag_of(xs) +# bag_of(ys)"
+apply (induct_tac "xs")
+apply (auto simp add: bag_of_multiset munion_assoc)
+done
+
+lemma bag_of_mono_aux [rule_format]:
+     "xs\<in>list(A) ==> \<forall>ys\<in>list(A). <xs, ys>\<in>prefix(A)  
+      --> <bag_of(xs), bag_of(ys)>\<in>MultLe(A, r)"
+apply (induct_tac "xs", simp_all, clarify) 
+apply (frule_tac l = ys in bag_of_multiset)
+apply (auto intro: empty_le_MultLe simp add: prefix_def)
+apply (rule munion_mono)
+apply (force simp add: MultLe_def Mult_iff_multiset)
+apply (blast dest: gen_prefix.dom_subset [THEN subsetD])
+done
+
+lemma bag_of_mono [intro]:
+     "[|  <xs, ys>\<in>prefix(A); xs\<in>list(A); ys\<in>list(A) |]
+      ==> <bag_of(xs), bag_of(ys)>\<in>MultLe(A, r)"
+apply (blast intro: bag_of_mono_aux)
+done
+
+lemma mono_bag_of [simp]: 
+     "mono1(list(A), prefix(A), Mult(A), MultLe(A,r), bag_of)"
+by (auto simp add:  mono1_def bag_of_type)
+
+
+subsection{*The function @{term msetsum}*}
+
+lemmas nat_into_Fin = eqpoll_refl [THEN [2] Fin_lemma]
+
+lemma list_Int_length_Fin: "l \<in> list(A) ==> C Int length(l) \<in> Fin(length(l))"
+apply (drule length_type)
+apply (rule Fin_subset)
+apply (rule Int_lower2)
+apply (erule nat_into_Fin)
+done
+
+
+
+lemma mem_Int_imp_lt_length:
+     "[|xs \<in> list(A); k \<in> C \<inter> length(xs)|] ==> k < length(xs)"
+apply (simp add: ltI)
+done
+
+
+lemma bag_of_sublist_lemma:
+     "[|C \<subseteq> nat; x \<in> A; xs \<in> list(A)|]   
+  ==>  msetsum(\<lambda>i. {#nth(i, xs @ [x])#}, C \<inter> succ(length(xs)), A) =  
+       (if length(xs) \<in> C then  
+          {#x#} +# msetsum(\<lambda>x. {#nth(x, xs)#}, C \<inter> length(xs), A)  
+        else msetsum(\<lambda>x. {#nth(x, xs)#}, C \<inter> length(xs), A))"
+apply (simp add: subsetD nth_append lt_not_refl mem_Int_imp_lt_length cong add: msetsum_cong)
+apply (simp add: Int_succ_right)
+apply (simp add: lt_not_refl mem_Int_imp_lt_length cong add: msetsum_cong, clarify)
+apply (subst msetsum_cons)
+apply (rule_tac [3] succI1)
+apply (blast intro: list_Int_length_Fin subset_succI [THEN Fin_mono, THEN subsetD])
+apply (simp add: mem_not_refl)
+apply (simp add: nth_type lt_not_refl)
+apply (blast intro: nat_into_Ord ltI length_type)
+apply (simp add: lt_not_refl mem_Int_imp_lt_length cong add: msetsum_cong)
+done
+
+lemma bag_of_sublist_lemma2:
+     "l\<in>list(A) ==>  
+  C <= nat ==>  
+  bag_of(sublist(l, C)) =  
+      msetsum(%i. {#nth(i, l)#}, C Int length(l), A)"
+apply (erule list_append_induct)
+apply (simp (no_asm))
+apply (simp (no_asm_simp) add: sublist_append nth_append bag_of_sublist_lemma munion_commute bag_of_sublist_lemma msetsum_multiset munion_0)
+done
+
+
+lemma nat_Int_length_eq: "l \<in> list(A) ==> nat \<inter> length(l) = length(l)"
+apply (rule Int_absorb1)
+apply (rule OrdmemD, auto)
+done
+
+(*eliminating the assumption C<=nat*)
+lemma bag_of_sublist:
+     "l\<in>list(A) ==>  
+  bag_of(sublist(l, C)) = msetsum(%i. {#nth(i, l)#}, C Int length(l), A)"
+apply (subgoal_tac " bag_of (sublist (l, C Int nat)) = msetsum (%i. {#nth (i, l) #}, C Int length (l), A) ")
+apply (simp add: sublist_Int_eq)
+apply (simp add: bag_of_sublist_lemma2 Int_lower2 Int_assoc nat_Int_length_eq)
+done
+
+lemma bag_of_sublist_Un_Int: 
+"l\<in>list(A) ==>  
+  bag_of(sublist(l, B Un C)) +# bag_of(sublist(l, B Int C)) =  
+      bag_of(sublist(l, B)) +# bag_of(sublist(l, C))"
+apply (subgoal_tac "B Int C Int length (l) = (B Int length (l)) Int (C Int length (l))")
+prefer 2 apply blast
+apply (simp (no_asm_simp) add: bag_of_sublist Int_Un_distrib2 msetsum_Un_Int)
+apply (rule msetsum_Un_Int)
+apply (erule list_Int_length_Fin)+
+ apply (simp add: ltI nth_type)
+done
+
+
+lemma bag_of_sublist_Un_disjoint:
+     "[| l\<in>list(A); B Int C = 0  |] 
+      ==> bag_of(sublist(l, B Un C)) =  
+          bag_of(sublist(l, B)) +# bag_of(sublist(l, C))"
+by (simp add: bag_of_sublist_Un_Int [symmetric] bag_of_multiset)
+
+
+lemma bag_of_sublist_UN_disjoint [rule_format]:
+     "[|Finite(I); \<forall>i\<in>I. \<forall>j\<in>I. i\<noteq>j --> A(i) \<inter> A(j) = 0;  
+        l\<in>list(B) |]  
+      ==> bag_of(sublist(l, \<Union>i\<in>I. A(i))) =   
+          (msetsum(%i. bag_of(sublist(l, A(i))), I, B)) "
+apply (simp (no_asm_simp) del: UN_simps
+           add: UN_simps [symmetric] bag_of_sublist)
+apply (subst  msetsum_UN_disjoint [of _ _ _ "length (l)"])
+apply (drule Finite_into_Fin, assumption)
+prefer 3 apply force
+apply (auto intro!: Fin_IntI2 Finite_into_Fin simp add: ltI nth_type length_type nat_into_Finite)
+done
+
+
+lemma part_ord_Lt [simp]: "part_ord(nat, Lt)"
+apply (unfold part_ord_def Lt_def irrefl_def trans_on_def)
+apply (auto intro: lt_trans)
+done
+
+subsubsection{*The function @{term all_distinct}*}
+
+lemma all_distinct_Nil [simp]: "all_distinct(Nil)"
+by (unfold all_distinct_def, auto)
+
+lemma all_distinct_Cons [simp]: 
+    "all_distinct(Cons(a,l)) <->  
+      (a\<in>set_of_list(l) --> False) & (a \<notin> set_of_list(l) --> all_distinct(l))"
+apply (unfold all_distinct_def)
+apply (auto elim: list.cases)
+done
+
+subsubsection{*The function @{term state_of}*}
+
+lemma state_of_state: "s\<in>state ==> state_of(s)=s"
+by (unfold state_of_def, auto)
+declare state_of_state [simp]
+
+
+lemma state_of_idem: "state_of(state_of(s))=state_of(s)"
+
+apply (unfold state_of_def, auto)
+done
+declare state_of_idem [simp]
+
+
+lemma state_of_type [simp,TC]: "state_of(s)\<in>state"
+by (unfold state_of_def, auto)
+
+lemma lift_apply [simp]: "lift(x, s)=s`x"
+by (simp add: lift_def)
+
+
+(** Used in ClientImp **)
+
+lemma gen_Increains_state_of_eq: 
+     "Increasing(A, r, %s. f(state_of(s))) = Increasing(A, r, f)"
+apply (unfold Increasing_def, auto)
+done
+
+lemmas Increasing_state_ofD1 =  
+      gen_Increains_state_of_eq [THEN equalityD1, THEN subsetD, standard]
+lemmas Increasing_state_ofD2 =  
+      gen_Increains_state_of_eq [THEN equalityD2, THEN subsetD, standard]
+
+lemma Follows_state_of_eq: 
+     "Follows(A, r, %s. f(state_of(s)), %s. g(state_of(s))) =   
+      Follows(A, r, f, g)"
+apply (unfold Follows_def Increasing_def, auto)
+done
+
+lemmas Follows_state_ofD1 =
+      Follows_state_of_eq [THEN equalityD1, THEN subsetD, standard]
+lemmas Follows_state_ofD2 =
+      Follows_state_of_eq [THEN equalityD2, THEN subsetD, standard]
+
+lemma nat_list_inj_type: "n\<in>nat ==> nat_list_inj(n)\<in>list(nat)"
+by (induct_tac "n", auto)
+
+lemma length_nat_list_inj: "n\<in>nat ==> length(nat_list_inj(n)) = n"
+by (induct_tac "n", auto)
+
+lemma var_infinite_lemma: 
+  "(\<lambda>x\<in>nat. nat_var_inj(x))\<in>inj(nat, var)"
+apply (unfold nat_var_inj_def)
+apply (rule_tac d = var_inj in lam_injective)
+apply (auto simp add: var.intros nat_list_inj_type)
+apply (simp add: length_nat_list_inj)
+done
+
+lemma nat_lepoll_var: "nat lepoll var"
+apply (unfold lepoll_def)
+apply (rule_tac x = " (\<lambda>x\<in>nat. nat_var_inj (x))" in exI)
+apply (rule var_infinite_lemma)
+done
+
+(*Surely a simpler proof uses lepoll_Finite and the following lemma:*)
+
+    (*????Cardinal*)
+    lemma nat_not_Finite: "~Finite(nat)"
+    apply (unfold Finite_def, clarify) 
+    apply (drule eqpoll_imp_lepoll [THEN lepoll_cardinal_le], simp) 
+    apply (insert Card_nat) 
+    apply (simp add: Card_def)
+    apply (drule le_imp_subset)
+    apply (blast elim: mem_irrefl)
+    done
+
+lemma var_not_Finite: "~Finite(var)"
+apply (insert nat_not_Finite) 
+apply (blast intro: lepoll_Finite [OF 	nat_lepoll_var]) 
+done
+
+lemma not_Finite_imp_exist: "~Finite(A) ==> \<exists>x. x\<in>A"
+apply (subgoal_tac "A\<noteq>0")
+apply (auto simp add: Finite_0)
+done
+
+lemma Inter_Diff_var_iff:
+     "Finite(A) ==> b\<in>(Inter(RepFun(var-A, B))) <-> (\<forall>x\<in>var-A. b\<in>B(x))"
+apply (subgoal_tac "\<exists>x. x\<in>var-A", auto)
+apply (subgoal_tac "~Finite (var-A) ")
+apply (drule not_Finite_imp_exist, auto)
+apply (cut_tac var_not_Finite)
+apply (erule swap)
+apply (rule_tac B = A in Diff_Finite, auto)
+done
+
+lemma Inter_var_DiffD:
+     "[| b\<in>Inter(RepFun(var-A, B)); Finite(A); x\<in>var-A |] ==> b\<in>B(x)"
+by (simp add: Inter_Diff_var_iff)
+
+(* [| Finite(A); (\<forall>x\<in>var-A. b\<in>B(x)) |] ==> b\<in>Inter(RepFun(var-A, B)) *)
+lemmas Inter_var_DiffI = Inter_Diff_var_iff [THEN iffD2, standard]
+
+declare Inter_var_DiffI [intro!]
+
+lemma Acts_subset_Int_Pow_simp [simp]:
+     "Acts(F)<= A \<inter> Pow(state*state)  <-> Acts(F)<=A"
+by (insert Acts_type [of F], auto)
+
+lemma setsum_nsetsum_eq: 
+     "[| Finite(A); \<forall>x\<in>A. g(x)\<in>nat |] 
+      ==> setsum(%x. $#(g(x)), A) = $# nsetsum(%x. g(x), A)"
+apply (erule Finite_induct)
+apply (auto simp add: int_of_add)
+done
+
+lemma nsetsum_cong: 
+     "[| A=B;  \<forall>x\<in>A. f(x)=g(x);  \<forall>x\<in>A. g(x)\<in>nat;  Finite(A) |]  
+      ==> nsetsum(f, A) = nsetsum(g, B)"
+apply (subgoal_tac "$# nsetsum (f, A) = $# nsetsum (g, B)", simp)
+apply (simp add: setsum_nsetsum_eq [symmetric] cong: setsum_cong) 
+done
 
 end
